Phi_System/Phi_Types.thy
@@ -2047,6 +2047,8 @@ declare [[\<phi>trace_reasoning = 0]]
        and \<open>homo_one \<delta>
         \<Longrightarrow> Tyops_Commute \<DD>[(\<circ>) \<delta>] \<DD>[\<delta>] ((\<^bold>\<rightarrow>) k) ((\<^bold>\<rightarrow>) k) Ta (\<lambda>_. True) (embedded_func (\<lambda>x. x) (\<lambda>_. True)) \<close>
 
+\<phi>adhoc_overloading \<phi>coercion \<open>\<lambda>T. [] \<^bold>\<rightarrow> T\<close>
+
 ML \<open>assert_derived_properties \<^theory> [
   (@{thm' \<phi>MapAt.Abstract_Domain\<^sub>L}, \<^pattern_prop>\<open> Abstract_Domain\<^sub>L ?T ?P \<Longrightarrow> Abstract_Domain\<^sub>L (?k \<^bold>\<rightarrow> ?T) ?P \<close>),
   (@{thm' \<phi>MapAt.Abstract_Domain}, \<^pattern_prop>\<open> Abstract_Domain ?T ?P \<Longrightarrow> Abstract_Domain (?k \<^bold>\<rightarrow> ?T) ?P \<close>),
@@ -2348,7 +2350,7 @@ declare [[\<phi>trace_reasoning = 0]]
        and Functional_Transformation_Functor
        and Abstraction_to_Raw
 
-\<phi>adhoc_overloading \<phi>coercion \<open>\<lambda>T. \<black_circle> Nosep T\<close> \<open>\<lambda>T. \<fish_eye> Nosep T\<close> (* \<open>\<lambda>T. \<fish_eye>\<^sub>L Nosep T\<close> *)
+\<phi>adhoc_overloading \<phi>coercion \<open>\<lambda>T. \<black_circle> Nosep T\<close> \<open>\<lambda>T. \<fish_eye> Nosep T\<close> \<open>\<lambda>T. \<fish_eye>\<^sub>L Nosep T\<close>
 
 ML \<open>assert_derived_properties \<^theory> [
   (@{thm' Nosep.Abstract_Domain\<^sub>L}, \<^pattern_prop>\<open> Abstract_Domain\<^sub>L ?T ?P \<Longrightarrow> Abstract_Domain\<^sub>L (Nosep ?T) ?P  \<close>),
@@ -2729,7 +2731,7 @@ lemma [\<phi>reason 1100]:
 
 lemma [\<phi>reason 1000]:
   \<open> x \<Ztypecolon> T \<t>\<r>\<a>\<n>\<s>\<f>\<o>\<r>\<m>\<s> y \<Ztypecolon> U \<w>\<i>\<t>\<h> P @action as Z
-\<Longrightarrow> x \<Ztypecolon> Agreement T \<t>\<r>\<a>\<n>\<s>\<f>\<o>\<r>\<m>\<s> y \<Ztypecolon> Agreement U \<w>\<i>\<t>\<h> P @action as Z\<close>
+\<Longrightarrow> x \<Ztypecolon> Agreement T \<t>\<r>\<a>\<s>\<f>\<o>\<r>\<m>\<s> y \<Ztypecolon> Agreement U \<w>\<i>\<t>\<h> P @action as Z\<close>
   unfolding Action_Tag_def using Agreement_cast .
 
 lemma [\<phi>reason 1100]:
